nola/examples/logic/intp.v
@@ -21,7 +21,13 @@ Section ncintp.
 
   (** Interpret basic connectives *)
   Definition ncintp0 (c : ncon0) : iProp Σ :=
-    match c with ⟨⌜φ⌝⟩%nc => ⌜φ⌝ end.
+    match c with
+    | ⟨⌜φ⌝⟩%nc => ⌜φ⌝
+    | ⟨↦{dq}|l,v⟩%nc => l ↦{dq} v
+    | ⟨↦_J|l,v⟩%nc => l ↦_J v
+    | ⟨↦□_J|l⟩%nc => l ↦_J □
+    | nc_meta_token l E => meta_token l E
+    end.
   Definition ncintpl0 (c : nconl0) (niS : nPropS (;ᵞ) → iProp Σ) : iProp Σ :=
     match c with nc_inv_wsat => ninv_wsat niS end.
   Definition ncintp1 (c : ncon1) (P : iProp Σ) : iProp Σ :=
